\chapter{Vector Function}
\section{Vector Function}
\subsection{Definition}
Basic form for vector function:
\begin{center}
$\mathbf{v}(t)=\langle f(t),g(t),h(t)\rangle=f(t)\mathbf{\hat{i}}+g(t)\mathbf{\hat{j}}+h(t)\mathbf{\hat{k}}$
\end{center}

\subsection{Limit}
\begin{center}
$\displaystyle	\lim_{t \to t_0} \mathbf{v}(t) = \langle\displaystyle\lim_{t \to t_0}f(t),\displaystyle\lim_{t \to t_0}g(t),\displaystyle\lim_{t \to t_0}h(t)	\rangle$\\
$=\displaystyle\lim_{t \to t_0}f(t)\mathbf{\hat{i}}+\displaystyle\lim_{t \to t_0}g(t)\mathbf{\hat{j}}+\displaystyle\lim_{t \to t_0}h(t)\mathbf{\hat{k}}$
\end{center}

\subsection{Continuity}
$\mathbf{v}(t)$ is continuous at $t=t_0$, iff $\mathbf{v}(t_0)$ is defined.\\
Criteria for the continuity:
\begin{itemize}
\item $\displaystyle\lim_{t \to t_0} \mathbf{v}(t)$ exist
\item $\displaystyle\lim_{t \to t_0} \mathbf{v}(t)=\mathbf{v}(t_0)$
\end{itemize}

\subsection{Derivative}
\begin{center}
$\frac{\mathrm d}{\mathrm d t}\mathbf{v}(t)=\mathbf{v}'(t)=\langle f'(t),g'(t),h'(t) \rangle$\\
$=\frac{\mathrm d}{\mathrm d t}f(t)\mathbf{\hat{i}}+\frac{\mathrm d}{\mathrm d t}g(t)\mathbf{\hat{j}}+\frac{\mathrm d}{\mathrm d t}h(t)\mathbf{\hat{k}}$
\end{center}

\subsection{Operating Rules}
\begin{itemize}
\item $\frac{\mathrm d}{\mathrm d t}(\mathbf{v}(t)\pm \mathbf{w}(t))=\frac{\mathrm d}{\mathrm d t}\mathbf{v}(t)\pm \frac{\mathrm d}{\mathrm d t}\mathbf{w}(t)$
\item $\frac{\mathrm d}{\mathrm d t}[c(t)\mathbf{v}(t)]=[\frac{\mathrm d}{\mathrm d t}c(t)]\mathbf{v}(t)+c(t)\frac{\mathrm d}{\mathrm d t}\mathbf{v}(t)$
\item $\frac{\mathrm d}{\mathrm d t}(\mathbf{v}(t)\cdot \mathbf{w}(t))=\frac{\mathrm d}{\mathrm d t}\mathbf{v}(t)\cdot \mathbf{w}+\mathbf{v}(t)\cdot \frac{\mathrm d}{\mathrm d t}\mathbf{w}(t)$
\item $\frac{\mathrm d}{\mathrm d t}(\mathbf{v}(t)\times \mathbf{w}(t))=\frac{\mathrm d}{\mathrm d t}\mathbf{v}(t)\times \mathbf{w}+\mathbf{v}(t)\times \frac{\mathrm d}{\mathrm d t}\mathbf{w}(t)$
\item $\frac{\mathrm d}{\mathrm d t}\mathbf{v}(c(t))=\mathbf{v}'(c(t))c'(t)$
\end{itemize}

\subsection{Integration}
\begin{center}
$\displaystyle\int\limits_a^b \mathbf{v}(t)dt=\displaystyle\int\limits_a^b f(t)dt \mathbf{\hat{i}}+\displaystyle\int\limits_a^b g(t)dt \mathbf{\hat{j}}+\displaystyle\int\limits_a^b h(t)dt \mathbf{\hat{k}}$
\end{center}
Also similar to the principle of definite integral:\\
If $\mathbf{V}'(t)=\mathbf{v}(t)$, then
\begin{center}
$\displaystyle\int\limits_a^b \mathbf{v}(t)dt=\mathbf{V}(t) |_{a}^b$
\end{center}
\subsection{Parameter Representation a tangent line of a space curve}
\begin{center}
$\vec{\tau}(t)=\displaystyle\lim_{\Delta t\to 0}\frac{\vec{r}(t+\Delta t)-\vec{r}(t)}{\Delta t} $
\end{center}
For convenience, we choose to get the unit vector of the tangent vector 
\[
\hat{\tau }(t)=\frac{\vec{\tau }(t)}{|\vec{\tau }(t)|}
\]
%\begin{center}
%$$
%\end{center}

\subsection{Arc Length and Curvature}
Given a curve $\mathcal{C}$: $x=x(t)\quad y=y(t)\quad z=z(t)$, for small $\Delta t$: the length between two points can be approximated as the distance between two points, thus we have the following formula:
\begin{align*}
\Delta\mathcal{L} & = \sqrt{|\mathbf{r}(t+\Delta t)-\mathbf{r}(t)|^2}\\
& =\sqrt{(x(t+\Delta t)-x(t))^2+(y(t+\Delta t)-y(t))^2+(z(t+\Delta t)-z(t))^2}
\end{align*}

\begin{align*}
\lim_{\Delta t \to 0}\frac{\Delta\mathcal{L}}{\Delta t} &= \sqrt{|\mathbf{r}(t+\Delta t)-\mathbf{r}(t)|^2}	\\
&= \sqrt{\frac{(x(t+\Delta t)-x(t))^2}{\Delta t^2}+\frac{(y(t+\Delta t)-y(t))^2}{\Delta t^2}+\frac{(z(t+\Delta t)-z(t))^2}{\Delta t^2}}		\\
&\iff \displaystyle\lim_{\Delta t}\frac{\mathcal{L}(t+\Delta t)-\mathcal{L}(t)}{\Delta t}=\sqrt{x'^2(t)+y'^2(t)+z'^2(t)}=\frac{d\mathcal{L}}{dt}
\end{align*}

Therefore, we can express the arc length in the differentiation form:

\begin{equation}
\boxed{d\mathcal{L}=\sqrt{x'^2(t)+y'^2(t)+z'^2(t)}dt}
\end{equation}

If we reconsider the tangent vector $\overrightarrow{\tau }(t)$,

\begin{center}
$\overrightarrow{\tau }(t)=x'(t)\mathbf{\hat{i}}+y'(t)\mathbf{\hat{j}}+z'(t)\mathbf{\hat{k}}=\mathbf{r}'(t)$\\
$\frac{d\mathcal{L}}{dt}=\sqrt{x'^2(t)\mathbf{\hat{i}}^2+y'^2(t)\mathbf{\hat{j}}^2+z'^2(t)\mathbf{\hat{k}}^2}=|\mathbf{r}'(t)|$
\end{center}

therefore, we have the formula for the arc length:

\begin{equation}
\boxed{\mathcal{L}=s(t)=\displaystyle\int\limits_{t_0}^t|\overrightarrow{\tau }(t)|dt=\displaystyle\int\limits_{t_0}^t|\mathbf{r}'(t)|dt}
\end{equation}

In this way, we can see that $\mathcal{L}=s(t)$ is a function of $t$, suppose that the inverse function exist $t=t(s)$, we can rewrite the curve with respect to $s$:
\begin{center}
$x=x(t)=x(t(s))=X(s)$\\
$y=y(t)=y(t(s))=Y(s)$\\
$z=z(t)=z(t(s))=Z(s)$
\end{center}
as that $s$ is the parameter instead of $t$:
\begin{center}
$\mathcal{L}=s(t)=\displaystyle\int\limits_{t_0}^t|\mathbf{r}'(t(s)|dt \qquad \frac{ds}{dt}=|\mathbf{r}'(t)|$\\
$\implies \frac{d\mathbf{r}(t(s))}{dt}=\frac{d\mathbf{r}}{ds}\frac{ds}{dt}=|\mathbf{r}'(t)|\frac{d\mathbf{r}}{ds}$\\
$\implies \frac{1}{|\mathbf{r}'(t)|}\frac{d\mathbf{r}}{dt}=\frac{d\mathbf{r}}{ds}$\\
\end{center}
\begin{equation}
\boxed{\implies \hat{\tau}(t)=\frac{d\mathbf{r}}{ds}}
\end{equation}
\subsection{Curvature}
Definition:\\
Supposing that $\hat{\tau}$ is the unit tangent vector of the curve $\mathcal{C}$, then the curvature is:
\begin{equation}
\boxed{		\kappa=\left| \frac{d\hat{\tau}}{ds} \right|	=	\left|\frac{\frac{d\hat{\tau}}{dt}}{\frac{ds}{dt}}\right|	=	\left|\frac{\hat{\tau}'(t)}{\mathbf{r}'(t)}\right|	}
\end{equation}

We want to use $\mathbf{r}(t)$ to represent $\hat{\tau}'(t)$, so consider:

\begin{center}
$\mathbf{r}'(t)=|\mathbf{r}'(t)|\hat{\tau}(t)=\frac{ds}{dt}\hat{\tau}(t)$\\
$\mathbf{r}''(t)=\frac{d^2s}{dt^2}\hat{\tau}(t)+\frac{ds}{dt}\hat{\tau}'(t)$\\
$\mathbf{r}'(t)\times \mathbf{r}''(t)=(\frac{ds}{dt})^2(\hat{\tau}(t)\times \hat{\tau}'(t))$\\
$|\mathbf{r}'(t)\times \mathbf{r}''(t)|=|(\frac{ds}{dt})^2||(\hat{\tau}\times \hat{\tau}'|=|(\frac{ds}{dt})^2||\hat{\tau}||\hat{\tau}'|=|(\frac{ds}{dt})^2||\hat{\tau}'|$
\end{center}

Thus,

\begin{equation}
\boxed{|\hat{\tau}'|=\frac{|\mathbf{r}'(t)\times \mathbf{r}''(t)|}{(\frac{ds}{dt})^2}=\frac{|\mathbf{r}'(t)\times \mathbf{r}''(t)|}{|\mathbf{r}'(t)|^2}}
\end{equation}
Therefore:
\begin{equation}
\boxed{\kappa=\frac{|\hat{\tau}'(t)|}{|\mathbf{r}'(t)|}=\frac{|\mathbf{r}'(t)\times \mathbf{r}''(t)|}{|\mathbf{r}'(t)|^3}}
\end{equation}
Note that:\\
for higher dimension general case, this equation always holds true.\\ \\
For $1$-dimensional special case:
\begin{equation}
\boxed{\kappa=\frac{|f''(x)|}{[1+(f'(x))^2]^{\frac{3}{2}}}}
\end{equation}
\subsection{The Normal and Binormal Vectors}
The principle unit normal vector:
\begin{center}
$\mathbf{N}(t)=\frac{\hat{\tau}'(t)}{|\hat{\tau}'(t)|}$
\end{center}
Osculating plane: the plane that $\hat{\tau}(t)$ and $\mathbf{N}(t)$ span out.\\
Osculating circle: the approximation of the curve by circle with the radius $\rho = \frac{1}{\kappa}$\\
The binormal vector:
\begin{center}
$\mathbf{B}(t)=\hat{\tau}(t)\times \mathbf{N}(t)$
\end{center}
Normal plane: the plane that $\mathbf{B}(t)$ and $\mathbf{N}(t)$ span out.